kernel/clr/lux_runtime.c
@@ -10,7 +10,7 @@
  * - $lux_release: BURN (release WHITE token, free if count==0)
  */
 
-#include "clr/clr-kernel/clr_pebble_integration.h"
+#include "clr-kernel/clr_pebble_integration.h"
 #include "dat.h"
 #include "error.h"
 #include "fns.h"
@@ -18,6 +18,8 @@
 #include "pebble.h"
 #include "portlib.h"
 #include "u.h"
+
+static clr_heap_t *lux_heap;
 
 /*
  * $lux_alloc - Allocate CIL object (LIME operation)
@@ -33,7 +35,6 @@
  */
 void *lux_alloc(ulong size, ulong type_token) {
   clr_object_t *obj;
-  clr_heap_t *heap;
   PebbleState *ps;
 
   /* Get/create CLR heap for current process */
@@ -42,24 +43,21 @@ void *lux_alloc(ulong size, ulong type_token) {
     error("lux_alloc: no pebble state");
 
   /* Allocate heap if this is first CIL allocation */
-  if (up && up->clr_heap == nil) {
-    heap = mallocz(sizeof(clr_heap_t), 1);
-    if (heap == nil)
+  if (lux_heap == nil) {
+    lux_heap = mallocz(sizeof(clr_heap_t), 1);
+    if (lux_heap == nil)
       error(PEBBLE_E_NOMEM);
-    heap->pebble = ps;
-    heap->objects_head = nil;
-    heap->objects_tail = nil;
-    heap->object_count = 0;
-    up->clr_heap = heap;
-  } else {
-    heap = up ? up->clr_heap : nil;
+    lux_heap->pebble = ps;
+    lux_heap->objects_head = nil;
+    lux_heap->objects_tail = nil;
+    lux_heap->object_count = 0;
   }
 
-  if (heap == nil)
+  if (lux_heap == nil)
     error("lux_alloc: no CLR heap");
 
   /* Allocate object via Pebble (LIME: BLACK + WHITE) */
-  obj = clr_object_alloc(heap, size, CLR_TYPE_OBJECT);
+  obj = clr_object_alloc(lux_heap, size, CLR_REF);
   if (obj == nil)
     error(PEBBLE_E_NOMEM);
 
@@ -80,31 +78,29 @@ void *lux_alloc(ulong size, ulong type_token) {
  */
 void *lux_addref(void *ptr) {
   clr_object_t *obj;
-  clr_heap_t *heap;
   PebbleWhite *white;
 
   if (ptr == nil)
     return nil; /* Null references don't need refcount */
 
-  heap = up ? up->clr_heap : nil;
-  if (heap == nil)
+  if (lux_heap == nil)
     error("lux_addref: no CLR heap");
 
   /* Find object by data pointer (reverse lookup) */
-  lock(&heap->objects_lock);
-  for (obj = heap->objects_head; obj != nil; obj = obj->next) {
+  lock(&lux_heap->objects_lock);
+  for (obj = lux_heap->objects_head; obj != nil; obj = obj->next) {
     if (obj->data == ptr) {
-      unlock(&heap->objects_lock);
+      unlock(&lux_heap->objects_lock);
 
       /* Issue new WHITE token (VANILLA) */
-      white = clr_object_addref(heap, obj);
+      white = clr_object_addref(lux_heap, obj);
       if (white == nil)
         error(PEBBLE_E_AGAIN);
 
       return ptr;
     }
   }
-  unlock(&heap->objects_lock);
+  unlock(&lux_heap->objects_lock);
 
   error("lux_addref: object not found");
   return nil;
@@ -121,21 +117,19 @@ void *lux_addref(void *ptr) {
  */
 void lux_release(void *ptr) {
   clr_object_t *obj;
-  clr_heap_t *heap;
   PebbleWhite *white;
 
   if (ptr == nil)
     return; /* Null references don't need release */
 
-  heap = up ? up->clr_heap : nil;
-  if (heap == nil)
+  if (lux_heap == nil)
     error("lux_release: no CLR heap");
 
   /* Find object by data pointer */
-  lock(&heap->objects_lock);
-  for (obj = heap->objects_head; obj != nil; obj = obj->next) {
+  lock(&lux_heap->objects_lock);
+  for (obj = lux_heap->objects_head; obj != nil; obj = obj->next) {
     if (obj->data == ptr) {
-      unlock(&heap->objects_lock);
+      unlock(&lux_heap->objects_lock);
 
       /* Find any WHITE token for this object */
       lock(&obj->lock);
@@ -148,7 +142,7 @@ void lux_release(void *ptr) {
 
         if (white) {
           /* Release white token (BURN) */
-          clr_object_release(heap, obj, white);
+          clr_object_release(lux_heap, obj, white);
           /* Note: clr_object_release frees obj if white_count==0 */
         }
       } else {
@@ -158,9 +152,52 @@ void lux_release(void *ptr) {
       return;
     }
   }
-  unlock(&heap->objects_lock);
+  unlock(&lux_heap->objects_lock);
 
   /* Not found - could be already freed, just ignore */
+}
+
+/*
+ * $lux_snapshot - Create Red snapshot for transactional semantics
+ */
+void *lux_snapshot(void *ptr) {
+  if (ptr == nil)
+    return nil;
+
+  PebbleState *ps = pebble_state();
+  if (ps == nil)
+    return ptr;
+
+  PebbleBlue *blue = nil;
+  for (PebbleBlue *b = ps->blue_list; b != nil; b = b->next) {
+    if (b->blue_data == ptr) {
+      blue = b;
+      break;
+    }
+  }
+
+  if (blue == nil)
+    return ptr;
+
+  PebbleRed *red = nil;
+  if (pebble_red_snapshot(blue, &red) != 0)
+    return ptr;
+
+  return red ? red->red_data : ptr;
+}
+
+/*
+ * $lux_commit - Commit transactional changes (MVP no-op)
+ */
+void lux_commit(void *ptr) {
+  USED(ptr);
+}
+
+/*
+ * $lux_rollback - Rollback transactional changes (MVP no-op)
+ */
+void lux_rollback(void *ptr) {
+  USED(ptr);
 }
 
 /*
