kernel/clr/wasm_backend/cil_to_wasm.h
@@ -1,0 +1,9 @@
+#ifndef CIL_TO_WASM_H
+#define CIL_TO_WASM_H
+
+#include "../il_parser.h"
+#include "wasm_buffer.h"
+
+int cil_to_wasm_compile_method(il_method_t *method, wasm_buffer_t *buf);
+
+#endif
