kernel/include/types_fwd.h
@@ -1,0 +1,53 @@
+/*
+ * Kernel Forward Type Declarations
+ *
+ * Centralized forward declarations for core kernel types.
+ * Include this header when you need type names but not full definitions.
+ */
+
+#ifndef _TYPES_FWD_H_
+#define _TYPES_FWD_H_
+
+/* Process type */
+#ifndef _PROC_DEFINED
+#define _PROC_DEFINED
+typedef struct Proc Proc;
+#endif
+
+/* Machine/CPU type */
+#ifndef _MACH_DEFINED
+#define _MACH_DEFINED
+typedef struct Mach Mach;
+#endif
+
+/* Lock type */
+#ifndef _LOCK_DEFINED
+#define _LOCK_DEFINED
+typedef struct Lock Lock;
+#endif
+
+/* Channel type */
+#ifndef _CHAN_DEFINED
+#define _CHAN_DEFINED
+typedef struct Chan Chan;
+#endif
+
+/* 9P message type */
+#ifndef _FCALL_DEFINED
+#define _FCALL_DEFINED
+typedef struct Fcall Fcall;
+#endif
+
+/* User registers type */
+#ifndef _UREG_DEFINED
+#define _UREG_DEFINED
+typedef struct Ureg Ureg;
+#endif
+
+/* Rendezvous type */
+#ifndef _RENDEZ_DEFINED
+#define _RENDEZ_DEFINED
+typedef struct Rendez Rendez;
+#endif
+
+#endif /* _TYPES_FWD_H_ */
