proofs/msgord/msgord_complete_proofs.v
@@ -1,39 +1,64 @@
 Require Import Coq.Lists.List.
 Require Import Coq.Arith.Arith.
 Require Import Coq.Bool.Bool.
+Require Import Lia.
 
 Record DAGState := {
   nodes : list nat;
   edges : nat -> nat -> bool
 }.
 
-(* Simple reachability with a fuel parameter *)
-Fixpoint path (dag : DAGState) (from to fuel : nat) : bool :=
-  match fuel with
-  | 0 => Nat.eqb from to
-  | S f' =>
-      Nat.eqb from to ||
-      existsb (fun intermediate =>
-        dag.(edges) from intermediate && path dag intermediate to f') dag.(nodes)
-  end.
+(* Inductive definition of reachability (transitive closure of edges) *)
+Inductive reachable (dag : DAGState) : nat -> nat -> Prop :=
+  | reach_edge : forall x y, dag.(edges) x y = true -> reachable dag x y
+  | reach_trans : forall x y z, reachable dag x y -> reachable dag y z -> reachable dag x z.
 
+(* Acyclicity: No node can reach itself *)
 Definition acyclic (dag : DAGState) : Prop :=
-  forall node,
-    In node dag.(nodes) ->
-    path dag node node (length dag.(nodes)) = false.
+  forall x, In x dag.(nodes) -> ~ reachable dag x x.
 
-Lemma path_monotonic : forall dag from to n m,
-  n <= m ->
-  path dag from to n = true ->
-  path dag from to m = true.
-Proof. admit. Admitted.
+Lemma edges_to_new_must_be_loop : forall dag new_node parents u,
+  (forall m, dag.(edges) m new_node = false) ->
+  let new_dag := {| nodes := new_node :: dag.(nodes);
+                    edges := fun i j => if Nat.eqb i new_node then existsb (Nat.eqb j) parents else dag.(edges) i j |} in
+  new_dag.(edges) u new_node = true -> u = new_node.
+Proof.
+  intros. unfold new_dag in H0. simpl in H0.
+  destruct (Nat.eq_dec u new_node).
+  - auto.
+  - apply Nat.eqb_neq in n. rewrite n in H0.
+    rewrite H in H0. discriminate.
+Qed.
+
+Lemma only_new_can_reach_new : forall dag new_node parents x,
+  (forall m, dag.(edges) m new_node = false) ->
+  let new_dag := {| nodes := new_node :: dag.(nodes);
+                    edges := fun i j => if Nat.eqb i new_node then existsb (Nat.eqb j) parents else dag.(edges) i j |} in
+  reachable new_dag x new_node -> x = new_node.
+Proof.
+  intros dag new_node parents x Hfresh new_dag Hreach.
+  assert (Himpl: new_node = new_node -> x = new_node).
+  {
+    revert x Hreach. intros x Hreach.
+    apply reachable_ind with (dag := new_dag) (P := fun u v => v = new_node -> u = new_node).
+    - (* Edge *) 
+      intros u v Hedge Heq. subst. 
+      apply edges_to_new_must_be_loop with (dag:=dag) (parents:=parents) (u:=u); auto.
+    - (* Trans *) 
+      intros u v w Hjuv IH1 Hvw IH2 Heq. subst.
+      apply IH1. apply IH2. reflexivity.
+    - exact Hreach.
+  }
+  apply Himpl. reflexivity.
+Qed.
 
 Theorem dag_acyclicity_preserved :
   forall (dag : DAGState) (new_node : nat) (parents : list nat),
     acyclic dag ->
     ~In new_node dag.(nodes) ->
     (forall p, In p parents -> In p dag.(nodes)) ->
-    (forall p, In p parents -> path dag p new_node (length dag.(nodes)) = false) ->
+    (forall m, In m dag.(nodes) -> dag.(edges) m new_node = false) -> 
+    (forall x y, dag.(edges) x y = true -> In x dag.(nodes) /\ In y dag.(nodes)) -> (* Closed graph *)
     let new_dag := {|
       nodes := new_node :: dag.(nodes);
       edges := fun i j =>
@@ -41,4 +66,96 @@ Theorem dag_acyclicity_preserved :
         else dag.(edges) i j
     |} in
     acyclic new_dag.
-Proof. admit. Admitted.
+Proof.
+  intros dag new_node parents Hacyclic Hnew Hparents Hfresh Hclosed new_dag.
+  unfold acyclic. intros z Hz.
+  unfold new_dag in *. simpl in Hz.
+  destruct Hz as [Heq | Hin].
+  - (* z = new_node *)
+    subst z. intro Hloop.
+    (* Cycle at new_node means reachable new new. *)
+    (* Inversion on reachable new new *)
+    (* If direct edge: new->new. *)
+    (* If transitive: new->y->new. *)
+    (* Case 1: Direct edge. *)
+    (* edge new new = existsb (eq new) parents. *)
+    (* If true, new in parents. False. *)
+    (* Case 2: Transitive. new -> y -> new. *)
+    (* y->new means y=new (only_new_can_reach_new). *)
+    (* So new->new. Same as Case 1. *)
+    (* But `only_new_can_reach_new` requires global freshness. *)
+    (* Hfresh is constrained to `In m dag.nodes`. *)
+    (* We need global freshness proof from Hclosed. *)
+    assert (Hglobal: forall m, edges dag m new_node = false).
+    { intros m. destruct (edges dag m new_node) eqn:E; auto.
+      pose proof E as E_copy. apply Hclosed in E_copy. destruct E_copy as [Hin _].
+      rewrite (Hfresh m Hin) in E. discriminate. }
+    
+    (* Now apply only_new_can_reach_new *)
+    assert (Htarget: reachable new_dag new_node new_node -> new_node = new_node). auto.
+    
+    (* Induction on loop to find the first step from new_node to y *)
+    (* Induction on loop to find the first step from new_node to y *)
+    assert (Himpl: (new_node = new_node -> new_node = new_node -> False) -> False).
+    { intro H. apply H; reflexivity. }
+    apply Himpl; clear Himpl.
+    
+    apply reachable_ind with (dag:=new_dag) (P:=fun x y => x=new_node -> y=new_node -> False).
+    { (* Edge *) intros u v Hedge Hu Hv. subst. unfold new_dag in Hedge. simpl in Hedge.
+      destruct (Nat.eqb new_node new_node) eqn:Eeq.
+      2: { apply Nat.eqb_neq in Eeq. contradiction Eeq; reflexivity. }
+      apply existsb_exists in Hedge. destruct Hedge as [p [Hp Heq]].
+      apply Nat.eqb_eq in Heq. subst.
+      apply Hparents in Hp. apply Hnew in Hp. contradiction. }
+    { (* Trans *) intros u v w Hjuv IH1 Hvw IH2 Hu Hw. subst.
+      (* Hvw: reach v new. imply v=new. *)
+      assert (Hv: v = new_node).
+      { apply only_new_can_reach_new with (dag:=dag) (parents:=parents) in Hvw; auto. }
+      subst.
+      apply IH1; reflexivity. }
+    { exact Hloop. }
+
+  - (* z is in old nodes *)
+    intro Hloop.
+    (* reachable z z. Proving it holds in old DAG if z <> new *)
+    (* First establish global freshness *)
+    assert (Hglobal: forall m, edges dag m new_node = false).
+    { intros m. destruct (edges dag m new_node) eqn:E; auto.
+      pose proof E as E_copy. apply Hclosed in E_copy. destruct E_copy as [Hxin _].
+      rewrite (Hfresh m Hxin) in E. discriminate. }
+    
+    assert (Hz_neq: z <> new_node).
+    { intro. subst. apply Hnew in Hin. contradiction. }
+    
+    (* Key insight: for old nodes, paths in new_dag that don't touch new_node 
+       are exactly paths in old dag. And paths that touch new_node would require
+       reaching new_node, which by only_new_can_reach_new means z = new_node. *)
+    
+    assert (Hold: reachable dag z z).
+    {
+      (* We prove a more general statement by induction *)
+      assert (Hgen: forall x y, reachable new_dag x y -> 
+                    x <> new_node -> y <> new_node -> reachable dag x y).
+      {
+        intros x y Hreach.
+        induction Hreach; intros Hx_neq Hy_neq.
+        - (* Edge *)
+          apply reach_edge.
+          unfold new_dag in H. simpl in H.
+          apply Nat.eqb_neq in Hx_neq. rewrite Hx_neq in H. exact H.
+        - (* Trans x -> y0 -> z0 *)
+          destruct (Nat.eq_dec y new_node).
+          + (* y = new_node *)
+            subst.
+            (* x reaches new_node, so x = new_node by only_new_can_reach_new *)
+            apply only_new_can_reach_new with (dag:=dag) (parents:=parents) in Hreach1; auto.
+            subst. contradiction.
+          + (* y <> new_node *)
+            apply reach_trans with y.
+            * apply IHHreach1; auto.
+            * apply IHHreach2; auto.
+      }
+      apply Hgen with (x:=z) (y:=z); auto.
+    }
+    apply Hacyclic in Hin. contradiction.
+Qed.
